src/lib/spec/Kuiper.Spec.Softmax.fsti
@@ -6,8 +6,17 @@ open Kuiper.Array1
 open Kuiper.Seq.Common
 
 (* Real-value golden specification for softmax. *)
-let softmax_real (s:Seq.seq real) =
+let softmax_real (s : seq real) =
   seq_mapi s (fun x i ->
     let exps = seq_map rexp s in
     let summ : real = rsum exps in
     rexp x /. summ)
+
+val shift_denom (r0 : Seq.seq real) (c : real)
+  : Lemma (ensures rsum (seq_map (fun z -> rexp (z -. c)) r0)
+                   == rsum (seq_map rexp r0) /. rexp c)
+
+(* Softmax is unchanged by a shift. *)
+val softmax_shift (r0 : seq real) (c : real)
+  : Lemma (ensures softmax_real (seq_map (fun x -> x -. c) r0)
+                   == softmax_real r0)
