src/lib/kernel/Kuiper.Kernel.Softmax.fsti
@@ -2,22 +2,20 @@ module Kuiper.Kernel.Softmax
 
 #lang-pulse
 open Kuiper
-open Kuiper.Real { rexp }
-open Kuiper.Seq.Common
-module Vec = Pulse.Lib.Vec
 open Kuiper.Array1
 open Kuiper.Tensor.Layout { ctlayout }
-open Kuiper.Tensor.Layout.Alg { l1_forward }
 open Kuiper.Spec.Softmax
+module Array1 = Kuiper.Array1
 
-unfold
-type softmax_gpu_ty (et : Type0) {| floating et, real_like et |} =
-  fn (nth : szp{nth <= max_threads})
-     (#lena : szp)
-     (#l : Kuiper.Array1.layout lena) {| ctlayout l |}
-     (a : array1 et l { is_global a })
-     (#va : erased (lseq et lena))
-     (ra : erased (lseq real lena))
+inline_for_extraction noextract
+fn softmax_gpu
+  (#et : Type0) {| floating et, real_like et, floating_real_like et |}
+  (nth : szp {nth <= max_threads})
+  (#lena : szp)
+  (#l : Array1.layout lena) {| ctlayout l |}
+  (a : array1 et l { is_global a })
+  (#va : erased (lseq et lena))
+  (ra : erased (lseq real lena))
   preserves
     cpu
   requires
@@ -28,30 +26,3 @@ type softmax_gpu_ty (et : Type0) {| floating et, real_like et |} =
     exists* (va' : lseq et lena).
       on gpu_loc (a |-> va') **
       pure (va' %~ softmax_real ra)
-
-unfold
-type softmax_ty (et : Type0) {| floating et, real_like et |} =
-  fn (nth : szp{nth <= max_threads})
-     (#lena : szp)
-     (a : Vec.lvec et lena)
-     (#va : erased (lseq et lena))
-     (ra : erased (lseq real lena))
-  preserves
-    cpu
-  requires
-    a |-> va **
-    pure (va %~ ra) **
-    pure (lena <= max_blocks * max_threads)
-    // ^ This could be removed
-  ensures
-    exists* (va' : lseq et lena).
-      a |-> va' **
-      pure (va' %~ softmax_real ra)
-
-inline_for_extraction noextract
-val softmax_gpu (#et : Type0) {| floating et, real_like et, floating_real_like et |}
-  : softmax_gpu_ty et
-
-inline_for_extraction noextract
-val softmax (#et : Type0) {| floating et, real_like et, floating_real_like et |}
-  : softmax_ty et
